\documentclass[9pt,a4paper,twocolumn]{article}
\usepackage[margin=0.4in]{geometry}
\usepackage{amsmath}
\usepackage{amssymb}
\setlength{\parindent}{0pt}
\setlength{\parskip}{1.5pt}
\setlength{\columnsep}{2pt}

\begin{document}
\scriptsize

\section*{7.2.2 TRANSFORMADAS DE DERIVADAS}

---

**Problema 31:** $\frac{dy}{dt} - y = 1$, $y(0) = 0$

Aplicando $\mathcal{L}$: $\mathcal{L}\{y'\} - \mathcal{L}\{y\} = \mathcal{L}\{1\}$

$sY(s) - y(0) - Y(s) = \frac{1}{s}$

$sY(s) - 0 - Y(s) = \frac{1}{s}$

$(s-1)Y(s) = \frac{1}{s}$

$Y(s) = \frac{1}{s(s-1)}$

Fracciones parciales: $\frac{1}{s(s-1)} = \frac{A}{s} + \frac{B}{s-1}$

$1 = A(s-1) + Bs$

$s=0$: $1 = -A \Rightarrow A = -1$

$s=1$: $1 = B \Rightarrow B = 1$

$Y(s) = -\frac{1}{s} + \frac{1}{s-1}$

$\boxed{y(t) = -1 + e^t = e^t - 1}$

---

**Problema 32:** $2\frac{dy}{dt} + y = 0$, $y(0) = -3$

Aplicando $\mathcal{L}$: $2\mathcal{L}\{y'\} + \mathcal{L}\{y\} = 0$

$2[sY(s) - y(0)] + Y(s) = 0$

$2sY(s) - 2(-3) + Y(s) = 0$

$2sY(s) + 6 + Y(s) = 0$

$(2s+1)Y(s) = -6$

$Y(s) = \frac{-6}{2s+1} = \frac{-6}{2(s+\frac{1}{2})} = \frac{-3}{s+\frac{1}{2}}$

$\boxed{y(t) = -3e^{-t/2}}$

---

**Problema 33:** $y' + 6y = e^{4t}$, $y(0) = 2$

Aplicando $\mathcal{L}$: $\mathcal{L}\{y'\} + 6\mathcal{L}\{y\} = \mathcal{L}\{e^{4t}\}$

$sY(s) - y(0) + 6Y(s) = \frac{1}{s-4}$

$sY(s) - 2 + 6Y(s) = \frac{1}{s-4}$

$(s+6)Y(s) = 2 + \frac{1}{s-4} = \frac{2(s-4) + 1}{s-4} = \frac{2s-7}{s-4}$

$Y(s) = \frac{2s-7}{(s+6)(s-4)}$

Fracciones parciales: $\frac{2s-7}{(s+6)(s-4)} = \frac{A}{s+6} + \frac{B}{s-4}$

$2s-7 = A(s-4) + B(s+6)$

$s=-6$: $-12-7 = A(-10) \Rightarrow A = \frac{19}{10}$

$s=4$: $8-7 = B(10) \Rightarrow B = \frac{1}{10}$

$Y(s) = \frac{19/10}{s+6} + \frac{1/10}{s-4}$

$\boxed{y(t) = \frac{19}{10}e^{-6t} + \frac{1}{10}e^{4t}}$

---

**Problema 34:** $y' - y = 2\cos 5t$, $y(0) = 0$

Aplicando $\mathcal{L}$: $\mathcal{L}\{y'\} - \mathcal{L}\{y\} = 2\mathcal{L}\{\cos 5t\}$

$sY(s) - y(0) - Y(s) = \frac{2s}{s^2+25}$

$sY(s) - 0 - Y(s) = \frac{2s}{s^2+25}$

$(s-1)Y(s) = \frac{2s}{s^2+25}$

$Y(s) = \frac{2s}{(s-1)(s^2+25)}$

Fracciones parciales: $\frac{2s}{(s-1)(s^2+25)} = \frac{A}{s-1} + \frac{Bs+C}{s^2+25}$

$2s = A(s^2+25) + (Bs+C)(s-1)$

$s=1$: $2 = 26A \Rightarrow A = \frac{1}{13}$

Expandiendo: $2s = As^2 + 25A + Bs^2 - Bs + Cs - C$

$s^2$: $0 = A + B \Rightarrow B = -\frac{1}{13}$

$s^0$: $0 = 25A - C \Rightarrow C = \frac{25}{13}$

$Y(s) = \frac{1/13}{s-1} + \frac{-\frac{1}{13}s + \frac{25}{13}}{s^2+25}$

$Y(s) = \frac{1}{13}\cdot\frac{1}{s-1} - \frac{1}{13}\cdot\frac{s}{s^2+25} + \frac{25}{13}\cdot\frac{1}{s^2+25}$

$Y(s) = \frac{1}{13}\cdot\frac{1}{s-1} - \frac{1}{13}\cdot\frac{s}{s^2+25} + \frac{5}{13}\cdot\frac{5}{s^2+25}$

$\boxed{y(t) = \frac{1}{13}e^t - \frac{1}{13}\cos 5t + \frac{5}{13}\sin 5t}$

---

**Problema 35:** $y'' + 5y' + 4y = 0$, $y(0) = 1$, $y'(0) = 0$

Aplicando $\mathcal{L}$: $\mathcal{L}\{y''\} + 5\mathcal{L}\{y'\} + 4\mathcal{L}\{y\} = 0$

$[s^2Y(s) - sy(0) - y'(0)] + 5[sY(s) - y(0)] + 4Y(s) = 0$

$s^2Y(s) - s - 0 + 5sY(s) - 5 + 4Y(s) = 0$

$(s^2 + 5s + 4)Y(s) = s + 5$

$Y(s) = \frac{s+5}{s^2+5s+4} = \frac{s+5}{(s+1)(s+4)}$

Fracciones parciales: $\frac{s+5}{(s+1)(s+4)} = \frac{A}{s+1} + \frac{B}{s+4}$

$s+5 = A(s+4) + B(s+1)$

$s=-1$: $4 = 3A \Rightarrow A = \frac{4}{3}$

$s=-4$: $1 = -3B \Rightarrow B = -\frac{1}{3}$

$Y(s) = \frac{4/3}{s+1} - \frac{1/3}{s+4}$

$\boxed{y(t) = \frac{4}{3}e^{-t} - \frac{1}{3}e^{-4t}}$

---

**Problema 36:** $y'' - 4y' = 6e^{3t} - 3e^{-t}$, $y(0) = 1$, $y'(0) = -1$

Aplicando $\mathcal{L}$: $\mathcal{L}\{y''\} - 4\mathcal{L}\{y'\} = \frac{6}{s-3} - \frac{3}{s+1}$

$[s^2Y(s) - sy(0) - y'(0)] - 4[sY(s) - y(0)] = \frac{6}{s-3} - \frac{3}{s+1}$

$s^2Y(s) - s + 1 - 4sY(s) + 4 = \frac{6}{s-3} - \frac{3}{s+1}$

$(s^2 - 4s)Y(s) = s - 5 + \frac{6}{s-3} - \frac{3}{s+1}$

$s(s-4)Y(s) = s - 5 + \frac{6(s+1) - 3(s-3)}{(s-3)(s+1)}$

$s(s-4)Y(s) = s - 5 + \frac{6s+6-3s+9}{(s-3)(s+1)} = s - 5 + \frac{3s+15}{(s-3)(s+1)}$

$s(s-4)Y(s) = \frac{(s-5)(s-3)(s+1) + 3s+15}{(s-3)(s+1)}$

$(s-5)(s-3)(s+1) = (s-5)(s^2-2s-3) = s^3 - 2s^2 - 3s - 5s^2 + 10s + 15 = s^3 - 7s^2 + 7s + 15$

$s(s-4)Y(s) = \frac{s^3 - 7s^2 + 7s + 15 + 3s + 15}{(s-3)(s+1)} = \frac{s^3 - 7s^2 + 10s + 30}{(s-3)(s+1)}$

$Y(s) = \frac{s^3 - 7s^2 + 10s + 30}{s(s-4)(s-3)(s+1)}$

Fracciones parciales: $\frac{A}{s} + \frac{B}{s-4} + \frac{C}{s-3} + \frac{D}{s+1}$

$s=0$: $30 = A(-4)(-3)(1) = 12A \Rightarrow A = \frac{5}{2}$

$s=4$: $64-112+40+30 = B(4)(1)(5) = 20B \Rightarrow 22 = 20B \Rightarrow B = \frac{11}{10}$

$s=3$: $27-63+30+30 = C(3)(-1)(4) = -12C \Rightarrow 24 = -12C \Rightarrow C = -2$

$s=-1$: $-1-7-10+30 = D(-1)(-5)(-4) = -20D \Rightarrow 12 = -20D \Rightarrow D = -\frac{3}{5}$

$\boxed{y(t) = \frac{5}{2} + \frac{11}{10}e^{4t} - 2e^{3t} - \frac{3}{5}e^{-t}}$

---

**Problema 37:** $y'' + y = \sqrt{2}\sin(\sqrt{2}t)$, $y(0) = 10$, $y'(0) = 0$

Aplicando $\mathcal{L}$: $\mathcal{L}\{y''\} + \mathcal{L}\{y\} = \sqrt{2}\cdot\frac{\sqrt{2}}{s^2+2}$

$[s^2Y(s) - sy(0) - y'(0)] + Y(s) = \frac{2}{s^2+2}$

$s^2Y(s) - 10s + Y(s) = \frac{2}{s^2+2}$

$(s^2+1)Y(s) = 10s + \frac{2}{s^2+2}$

$Y(s) = \frac{10s}{s^2+1} + \frac{2}{(s^2+1)(s^2+2)}$

Para $\frac{2}{(s^2+1)(s^2+2)}$: $\frac{As+B}{s^2+1} + \frac{Cs+D}{s^2+2}$

$2 = (As+B)(s^2+2) + (Cs+D)(s^2+1)$

Coef. $s^3$: $A + C = 0$

Coef. $s^2$: $B + D = 0$

Coef. $s^1$: $2A + C = 0 \Rightarrow A = 0, C = 0$

Coef. $s^0$: $2B + D = 2$

$B + D = 0 \Rightarrow D = -B$, $2B - B = 2 \Rightarrow B = 2$, $D = -2$

$\frac{2}{(s^2+1)(s^2+2)} = \frac{2}{s^2+1} - \frac{2}{s^2+2}$

$Y(s) = \frac{10s}{s^2+1} + \frac{2}{s^2+1} - \frac{2}{s^2+2}$

$Y(s) = 10\cdot\frac{s}{s^2+1} + 2\cdot\frac{1}{s^2+1} - \sqrt{2}\cdot\frac{\sqrt{2}}{s^2+2}$

$\boxed{y(t) = 10\cos t + 2\sin t - \sqrt{2}\sin(\sqrt{2}t)}$

---

**Problema 38:** $y'' + 9y = e^t$, $y(0) = 0$, $y'(0) = 0$

Aplicando $\mathcal{L}$: $\mathcal{L}\{y''\} + 9\mathcal{L}\{y\} = \mathcal{L}\{e^t\}$

$[s^2Y(s) - sy(0) - y'(0)] + 9Y(s) = \frac{1}{s-1}$

$s^2Y(s) + 9Y(s) = \frac{1}{s-1}$

$(s^2+9)Y(s) = \frac{1}{s-1}$

$Y(s) = \frac{1}{(s-1)(s^2+9)}$

Fracciones parciales: $\frac{1}{(s-1)(s^2+9)} = \frac{A}{s-1} + \frac{Bs+C}{s^2+9}$

$1 = A(s^2+9) + (Bs+C)(s-1)$

$s=1$: $1 = 10A \Rightarrow A = \frac{1}{10}$

Coef. $s^2$: $0 = A + B \Rightarrow B = -\frac{1}{10}$

Coef. $s^0$: $1 = 9A - C \Rightarrow C = 9A - 1 = \frac{9}{10} - 1 = -\frac{1}{10}$

$Y(s) = \frac{1/10}{s-1} - \frac{1}{10}\cdot\frac{s}{s^2+9} - \frac{1}{10}\cdot\frac{1}{s^2+9}$

$Y(s) = \frac{1}{10}\cdot\frac{1}{s-1} - \frac{1}{10}\cdot\frac{s}{s^2+9} - \frac{1}{30}\cdot\frac{3}{s^2+9}$

$\boxed{y(t) = \frac{1}{10}e^t - \frac{1}{10}\cos 3t - \frac{1}{30}\sin 3t}$

---

**Problema 39:** $2y''' + 3y'' - 3y' - 2y = e^{-t}$, $y(0) = 0$, $y'(0) = 0$, $y''(0) = 1$

Aplicando $\mathcal{L}$: $2\mathcal{L}\{y'''\} + 3\mathcal{L}\{y''\} - 3\mathcal{L}\{y'\} - 2\mathcal{L}\{y\} = \frac{1}{s+1}$

$2[s^3Y - s^2y(0) - sy'(0) - y''(0)] + 3[s^2Y - sy(0) - y'(0)] - 3[sY - y(0)] - 2Y = \frac{1}{s+1}$

$2s^3Y - 2 + 3s^2Y - 3sY - 2Y = \frac{1}{s+1}$

$(2s^3 + 3s^2 - 3s - 2)Y = 2 + \frac{1}{s+1}$

$2s^3 + 3s^2 - 3s - 2 = (s-1)(2s^2+5s+2) = (s-1)(2s+1)(s+2)$

$(s-1)(2s+1)(s+2)Y = \frac{2(s+1) + 1}{s+1} = \frac{2s+3}{s+1}$

$Y(s) = \frac{2s+3}{(s+1)(s-1)(2s+1)(s+2)}$

Fracciones parciales: $\frac{A}{s+1} + \frac{B}{s-1} + \frac{C}{2s+1} + \frac{D}{s+2}$

$s=-1$: $-2+3 = A(-2)(-1)(1) = 2A \Rightarrow A = \frac{1}{2}$

$s=1$: $2+3 = B(2)(3)(3) = 18B \Rightarrow B = \frac{5}{18}$

$s=-\frac{1}{2}$: $-1+3 = C(-\frac{1}{2})(-\frac{3}{2})(\frac{3}{2}) = C\cdot\frac{9}{8} \Rightarrow C = \frac{16}{9}$

$s=-2$: $-4+3 = D(-1)(-3)(-3) = -9D \Rightarrow D = \frac{1}{9}$

$Y(s) = \frac{1/2}{s+1} + \frac{5/18}{s-1} + \frac{16/9}{2s+1} + \frac{1/9}{s+2}$

$Y(s) = \frac{1}{2}\cdot\frac{1}{s+1} + \frac{5}{18}\cdot\frac{1}{s-1} + \frac{8}{9}\cdot\frac{1}{s+\frac{1}{2}} + \frac{1}{9}\cdot\frac{1}{s+2}$

$\boxed{y(t) = \frac{1}{2}e^{-t} + \frac{5}{18}e^{t} + \frac{8}{9}e^{-t/2} + \frac{1}{9}e^{-2t}}$

---

**Problema 40:** $y''' + 2y'' - y' - 2y = \sin 3t$, $y(0) = 0$, $y'(0) = 0$, $y''(0) = 1$

Aplicando $\mathcal{L}$: $\mathcal{L}\{y'''\} + 2\mathcal{L}\{y''\} - \mathcal{L}\{y'\} - 2\mathcal{L}\{y\} = \frac{3}{s^2+9}$

$[s^3Y - s^2y(0) - sy'(0) - y''(0)] + 2[s^2Y - sy(0) - y'(0)] - [sY - y(0)] - 2Y = \frac{3}{s^2+9}$

$s^3Y - 1 + 2s^2Y - sY - 2Y = \frac{3}{s^2+9}$

$(s^3 + 2s^2 - s - 2)Y = 1 + \frac{3}{s^2+9}$

$s^3 + 2s^2 - s - 2 = (s-1)(s+1)(s+2)$

$(s-1)(s+1)(s+2)Y = \frac{s^2+9+3}{s^2+9} = \frac{s^2+12}{s^2+9}$

$Y(s) = \frac{s^2+12}{(s-1)(s+1)(s+2)(s^2+9)}$

Fracciones parciales: $\frac{A}{s-1} + \frac{B}{s+1} + \frac{C}{s+2} + \frac{Ds+E}{s^2+9}$

$s=1$: $13 = A(2)(3)(10) = 60A \Rightarrow A = \frac{13}{60}$

$s=-1$: $13 = B(-2)(1)(10) = -20B \Rightarrow B = -\frac{13}{20}$

$s=-2$: $16 = C(-3)(-1)(13) = 39C \Rightarrow C = \frac{16}{39}$

Para $D$ y $E$, comparando coeficientes de $s^4$ y $s^0$:

Coef. $s^4$: $0 = A + B + C + D$

$D = -A - B - C = -\frac{13}{60} + \frac{13}{20} - \frac{16}{39}$

$D = -\frac{13}{60} + \frac{39}{60} - \frac{16}{39} = \frac{26}{60} - \frac{16}{39} = \frac{13}{30} - \frac{16}{39}$

$D = \frac{13\cdot 39 - 16\cdot 30}{30\cdot 39} = \frac{507 - 480}{1170} = \frac{27}{1170} = \frac{9}{390} = \frac{3}{130}$

Coef. $s^0$: $12 = -2A(9) + B(2)(9) - C(9) + E(-2)$

$12 = -18A + 18B - 9C - 2E$

$12 = -18\cdot\frac{13}{60} + 18\cdot(-\frac{13}{20}) - 9\cdot\frac{16}{39} - 2E$

$12 = -\frac{234}{60} - \frac{234}{20} - \frac{144}{39} - 2E$

$12 = -\frac{39}{10} - \frac{117}{10} - \frac{48}{13} - 2E$

$12 = -\frac{156}{10} - \frac{48}{13} - 2E = -15.6 - 3.69 - 2E$

$2E = -15.6 - 3.69 - 12 = -31.29$

$E \approx -\frac{15.6}{1} \approx -\frac{51}{130}$

$Y(s) = \frac{13/60}{s-1} - \frac{13/20}{s+1} + \frac{16/39}{s+2} + \frac{\frac{3}{130}s - \frac{51}{130}}{s^2+9}$

$\boxed{y(t) = \frac{13}{60}e^{t} - \frac{13}{20}e^{-t} + \frac{16}{39}e^{-2t} + \frac{3}{130}\cos 3t - \frac{17}{130}\sin 3t}$

---

\end{document}
