\documentclass[9pt,a4paper,twocolumn]{article}
\usepackage[margin=0.4in]{geometry}
\usepackage{amsmath}
\usepackage{amssymb}
\setlength{\parindent}{0pt}
\setlength{\parskip}{1.5pt}
\setlength{\columnsep}{2pt}

\begin{document}
\scriptsize

**Problema 1:** $\mathcal{L}^{-1}\left\{\frac{1}{s^3}\right\}$

Usando $\mathcal{L}\{t^n\} = \frac{n!}{s^{n+1}}$

Para $n = 2$: $\mathcal{L}\{t^2\} = \frac{2!}{s^3} = \frac{2}{s^3}$

$\frac{1}{s^3} = \frac{1}{2} \cdot \frac{2}{s^3}$

$\boxed{\mathcal{L}^{-1}\left\{\frac{1}{s^3}\right\} = \frac{t^2}{2}}$

---

**Problema 2:** $\mathcal{L}^{-1}\left\{\frac{1}{s^4}\right\}$

Usando $\mathcal{L}\{t^n\} = \frac{n!}{s^{n+1}}$

Para $n = 3$: $\mathcal{L}\{t^3\} = \frac{3!}{s^4} = \frac{6}{s^4}$

$\frac{1}{s^4} = \frac{1}{6} \cdot \frac{6}{s^4}$

$\boxed{\mathcal{L}^{-1}\left\{\frac{1}{s^4}\right\} = \frac{t^3}{6}}$

---

**Problema 3:** $\mathcal{L}^{-1}\left\{\frac{1}{s^2} - \frac{48}{s^5}\right\}$

$\mathcal{L}^{-1}\left\{\frac{1}{s^2}\right\} = t$ (ya que $\mathcal{L}\{t\} = \frac{1}{s^2}$)

$\mathcal{L}^{-1}\left\{\frac{48}{s^5}\right\}$: Para $n = 4$: $\mathcal{L}\{t^4\} = \frac{4!}{s^5} = \frac{24}{s^5}$

$\frac{48}{s^5} = 2 \cdot \frac{24}{s^5} \Rightarrow \mathcal{L}^{-1}\left\{\frac{48}{s^5}\right\} = 2t^4$

$\boxed{\mathcal{L}^{-1}\left\{\frac{1}{s^2} - \frac{48}{s^5}\right\} = t - 2t^4}$

---

**Problema 4:** $\mathcal{L}^{-1}\left\{\frac{2}{s} - \frac{1}{s^3}\right\}$

$\mathcal{L}^{-1}\left\{\frac{2}{s}\right\} = 2 \cdot \mathcal{L}^{-1}\left\{\frac{1}{s}\right\} = 2 \cdot 1 = 2$

$\mathcal{L}^{-1}\left\{\frac{1}{s^3}\right\} = \frac{t^2}{2}$ (del problema 1)

$\boxed{\mathcal{L}^{-1}\left\{\frac{2}{s} - \frac{1}{s^3}\right\} = 2 - \frac{t^2}{2}}$

---

**Problema 5:** $\mathcal{L}^{-1}\left\{\frac{(s+1)^3}{s^4}\right\}$

Expandiendo $(s+1)^3 = s^3 + 3s^2 + 3s + 1$

$\frac{(s+1)^3}{s^4} = \frac{s^3 + 3s^2 + 3s + 1}{s^4} = \frac{1}{s} + \frac{3}{s^2} + \frac{3}{s^3} + \frac{1}{s^4}$

$\mathcal{L}^{-1}\left\{\frac{1}{s}\right\} = 1$, $\mathcal{L}^{-1}\left\{\frac{3}{s^2}\right\} = 3t$

$\mathcal{L}^{-1}\left\{\frac{3}{s^3}\right\} = \frac{3t^2}{2}$, $\mathcal{L}^{-1}\left\{\frac{1}{s^4}\right\} = \frac{t^3}{6}$

$\boxed{\mathcal{L}^{-1}\left\{\frac{(s+1)^3}{s^4}\right\} = 1 + 3t + \frac{3t^2}{2} + \frac{t^3}{6}}$

---

**Problema 6:** $\mathcal{L}^{-1}\left\{\frac{(s+2)^2}{s^3}\right\}$

Expandiendo $(s+2)^2 = s^2 + 4s + 4$

$\frac{(s+2)^2}{s^3} = \frac{s^2 + 4s + 4}{s^3} = \frac{1}{s} + \frac{4}{s^2} + \frac{4}{s^3}$

$\mathcal{L}^{-1}\left\{\frac{1}{s}\right\} = 1$, $\mathcal{L}^{-1}\left\{\frac{4}{s^2}\right\} = 4t$, $\mathcal{L}^{-1}\left\{\frac{4}{s^3}\right\} = 2t^2$

$\boxed{\mathcal{L}^{-1}\left\{\frac{(s+2)^2}{s^3}\right\} = 1 + 4t + 2t^2}$

---

**Problema 7:** $\mathcal{L}^{-1}\left\{\frac{1}{s^2} - \frac{1}{s} + \frac{1}{s-2}\right\}$

$\mathcal{L}^{-1}\left\{\frac{1}{s^2}\right\} = t$, $\mathcal{L}^{-1}\left\{\frac{1}{s}\right\} = 1$, $\mathcal{L}^{-1}\left\{\frac{1}{s-2}\right\} = e^{2t}$

$\boxed{\mathcal{L}^{-1}\left\{\frac{1}{s^2} - \frac{1}{s} + \frac{1}{s-2}\right\} = t - 1 + e^{2t}}$

---

**Problema 8:** $\mathcal{L}^{-1}\left\{\frac{4}{s} - \frac{6}{s^5} + \frac{1}{s+8}\right\}$

$\mathcal{L}^{-1}\left\{\frac{4}{s}\right\} = 4$

$\mathcal{L}^{-1}\left\{\frac{6}{s^5}\right\} = 6 \cdot \frac{t^4}{24} = \frac{t^4}{4}$

$\mathcal{L}^{-1}\left\{\frac{1}{s+8}\right\} = e^{-8t}$

$\boxed{\mathcal{L}^{-1}\left\{\frac{4}{s} - \frac{6}{s^5} + \frac{1}{s+8}\right\} = 4 - \frac{t^4}{4} + e^{-8t}}$

---

**Problema 9:** $\mathcal{L}^{-1}\left\{\frac{1}{4s+1}\right\}$

$\frac{1}{4s+1} = \frac{1}{4(s+\frac{1}{4})} = \frac{1}{4} \cdot \frac{1}{s+\frac{1}{4}}$

$\mathcal{L}^{-1}\left\{\frac{1}{s+\frac{1}{4}}\right\} = e^{-t/4}$

$\boxed{\mathcal{L}^{-1}\left\{\frac{1}{4s+1}\right\} = \frac{1}{4}e^{-t/4}}$

---

**Problema 10:** $\mathcal{L}^{-1}\left\{\frac{1}{5s-2}\right\}$

$\frac{1}{5s-2} = \frac{1}{5(s-\frac{2}{5})} = \frac{1}{5} \cdot \frac{1}{s-\frac{2}{5}}$

$\mathcal{L}^{-1}\left\{\frac{1}{s-\frac{2}{5}}\right\} = e^{2t/5}$

$\boxed{\mathcal{L}^{-1}\left\{\frac{1}{5s-2}\right\} = \frac{1}{5}e^{2t/5}}$

---

**Problema 11:** $\mathcal{L}^{-1}\left\{\frac{5}{s^2+49}\right\}$

$\mathcal{L}\{\sin(at)\} = \frac{a}{s^2+a^2}$

$\frac{5}{s^2+49} = \frac{5}{s^2+7^2} = \frac{5}{7} \cdot \frac{7}{s^2+7^2}$

$\boxed{\mathcal{L}^{-1}\left\{\frac{5}{s^2+49}\right\} = \frac{5}{7}\sin(7t)}$

---

**Problema 12:** $\mathcal{L}^{-1}\left\{\frac{10s}{s^2+16}\right\}$

$\mathcal{L}\{\cos(at)\} = \frac{s}{s^2+a^2}$

$\frac{10s}{s^2+16} = 10 \cdot \frac{s}{s^2+4^2}$

$\boxed{\mathcal{L}^{-1}\left\{\frac{10s}{s^2+16}\right\} = 10\cos(4t)}$

---

**Problema 13:** $\mathcal{L}^{-1}\left\{\frac{4s}{4s^2+1}\right\}$

$\frac{4s}{4s^2+1} = \frac{4s}{4(s^2+\frac{1}{4})} = \frac{s}{s^2+(\frac{1}{2})^2}$

$\boxed{\mathcal{L}^{-1}\left\{\frac{4s}{4s^2+1}\right\} = \cos\left(\frac{t}{2}\right)}$

---

**Problema 14:** $\mathcal{L}^{-1}\left\{\frac{1}{4s^2+1}\right\}$

$\frac{1}{4s^2+1} = \frac{1}{4(s^2+\frac{1}{4})} = \frac{1}{4} \cdot \frac{1}{s^2+(\frac{1}{2})^2}$

$= \frac{1}{4} \cdot \frac{1}{\frac{1}{2}} \cdot \frac{\frac{1}{2}}{s^2+(\frac{1}{2})^2} = \frac{1}{2} \cdot \frac{\frac{1}{2}}{s^2+(\frac{1}{2})^2}$

$\boxed{\mathcal{L}^{-1}\left\{\frac{1}{4s^2+1}\right\} = \frac{1}{2}\sin\left(\frac{t}{2}\right)}$

---

**Problema 15:** $\mathcal{L}^{-1}\left\{\frac{2s-6}{s^2+9}\right\}$

$\frac{2s-6}{s^2+9} = \frac{2s}{s^2+9} - \frac{6}{s^2+9}$

$= 2 \cdot \frac{s}{s^2+3^2} - \frac{6}{3} \cdot \frac{3}{s^2+3^2} = 2 \cdot \frac{s}{s^2+3^2} - 2 \cdot \frac{3}{s^2+3^2}$

$\boxed{\mathcal{L}^{-1}\left\{\frac{2s-6}{s^2+9}\right\} = 2\cos(3t) - 2\sin(3t)}$

---

**Problema 16:** $\mathcal{L}^{-1}\left\{\frac{s+1}{s^2+2}\right\}$

$\frac{s+1}{s^2+2} = \frac{s}{s^2+(\sqrt{2})^2} + \frac{1}{s^2+(\sqrt{2})^2}$

$= \frac{s}{s^2+2} + \frac{1}{\sqrt{2}} \cdot \frac{\sqrt{2}}{s^2+2}$

$\boxed{\mathcal{L}^{-1}\left\{\frac{s+1}{s^2+2}\right\} = \cos(\sqrt{2}t) + \frac{1}{\sqrt{2}}\sin(\sqrt{2}t)}$

---

**Problema 17:** $\mathcal{L}^{-1}\left\{\frac{1}{s^2+3s}\right\}$

Fracciones parciales: $\frac{1}{s^2+3s} = \frac{1}{s(s+3)} = \frac{A}{s} + \frac{B}{s+3}$

$1 = A(s+3) + Bs$

$s = 0$: $1 = 3A \Rightarrow A = \frac{1}{3}$

$s = -3$: $1 = -3B \Rightarrow B = -\frac{1}{3}$

$\frac{1}{s^2+3s} = \frac{1}{3s} - \frac{1}{3(s+3)}$

$\boxed{\mathcal{L}^{-1}\left\{\frac{1}{s^2+3s}\right\} = \frac{1}{3} - \frac{1}{3}e^{-3t}}$

---

**Problema 18:** $\mathcal{L}^{-1}\left\{\frac{s+1}{s^2-4s}\right\}$

$\frac{s+1}{s^2-4s} = \frac{s+1}{s(s-4)} = \frac{A}{s} + \frac{B}{s-4}$

$s+1 = A(s-4) + Bs$

$s = 0$: $1 = -4A \Rightarrow A = -\frac{1}{4}$

$s = 4$: $5 = 4B \Rightarrow B = \frac{5}{4}$

$\boxed{\mathcal{L}^{-1}\left\{\frac{s+1}{s^2-4s}\right\} = -\frac{1}{4} + \frac{5}{4}e^{4t}}$

---

**Problema 19:** $\mathcal{L}^{-1}\left\{\frac{s}{s^2+2s-3}\right\}$

$s^2+2s-3 = (s+3)(s-1)$

$\frac{s}{(s+3)(s-1)} = \frac{A}{s+3} + \frac{B}{s-1}$

$s = A(s-1) + B(s+3)$

$s = -3$: $-3 = -4A \Rightarrow A = \frac{3}{4}$

$s = 1$: $1 = 4B \Rightarrow B = \frac{1}{4}$

$\boxed{\mathcal{L}^{-1}\left\{\frac{s}{s^2+2s-3}\right\} = \frac{3}{4}e^{-3t} + \frac{1}{4}e^{t}}$

---

**Problema 20:** $\mathcal{L}^{-1}\left\{\frac{1}{s^2+s-20}\right\}$

$s^2+s-20 = (s+5)(s-4)$

$\frac{1}{(s+5)(s-4)} = \frac{A}{s+5} + \frac{B}{s-4}$

$1 = A(s-4) + B(s+5)$

$s = -5$: $1 = -9A \Rightarrow A = -\frac{1}{9}$

$s = 4$: $1 = 9B \Rightarrow B = \frac{1}{9}$

$\boxed{\mathcal{L}^{-1}\left\{\frac{1}{s^2+s-20}\right\} = -\frac{1}{9}e^{-5t} + \frac{1}{9}e^{4t}}$

---

**Problema 21:** $\mathcal{L}^{-1}\left\{\frac{0.9s}{(s-0.1)(s+0.2)}\right\}$

$\frac{0.9s}{(s-0.1)(s+0.2)} = \frac{A}{s-0.1} + \frac{B}{s+0.2}$

$0.9s = A(s+0.2) + B(s-0.1)$

$s = 0.1$: $0.09 = 0.3A \Rightarrow A = 0.3$

$s = -0.2$: $-0.18 = -0.3B \Rightarrow B = 0.6$

$\boxed{\mathcal{L}^{-1}\left\{\frac{0.9s}{(s-0.1)(s+0.2)}\right\} = 0.3e^{0.1t} + 0.6e^{-0.2t}}$

---

**Problema 22:** $\mathcal{L}^{-1}\left\{\frac{s-3}{(s-\sqrt{3})(s+\sqrt{3})}\right\}$

$\frac{s-3}{s^2-3} = \frac{A}{s-\sqrt{3}} + \frac{B}{s+\sqrt{3}}$

$s-3 = A(s+\sqrt{3}) + B(s-\sqrt{3})$

$s = \sqrt{3}$: $\sqrt{3}-3 = 2\sqrt{3}A \Rightarrow A = \frac{\sqrt{3}-3}{2\sqrt{3}}$

$s = -\sqrt{3}$: $-\sqrt{3}-3 = -2\sqrt{3}B \Rightarrow B = \frac{\sqrt{3}+3}{2\sqrt{3}}$

$\boxed{\mathcal{L}^{-1}\left\{\frac{s-3}{s^2-3}\right\} = \frac{\sqrt{3}-3}{2\sqrt{3}}e^{\sqrt{3}t} + \frac{\sqrt{3}+3}{2\sqrt{3}}e^{-\sqrt{3}t}}$

---

**Problema 23:** $\mathcal{L}^{-1}\left\{\frac{s}{(s-2)(s-3)(s-6)}\right\}$

$\frac{s}{(s-2)(s-3)(s-6)} = \frac{A}{s-2} + \frac{B}{s-3} + \frac{C}{s-6}$

$s = A(s-3)(s-6) + B(s-2)(s-6) + C(s-2)(s-3)$

$s = 2$: $2 = A(-1)(-4) = 4A \Rightarrow A = \frac{1}{2}$

$s = 3$: $3 = B(1)(-3) = -3B \Rightarrow B = -1$

$s = 6$: $6 = C(4)(3) = 12C \Rightarrow C = \frac{1}{2}$

$\boxed{\mathcal{L}^{-1}\left\{\frac{s}{(s-2)(s-3)(s-6)}\right\} = \frac{1}{2}e^{2t} - e^{3t} + \frac{1}{2}e^{6t}}$

---

**Problema 24:** $\mathcal{L}^{-1}\left\{\frac{s^2+1}{s(s-1)(s+1)(s-2)}\right\}$

$\frac{s^2+1}{s(s-1)(s+1)(s-2)} = \frac{A}{s} + \frac{B}{s-1} + \frac{C}{s+1} + \frac{D}{s-2}$

$s = 0$: $1 = A(-1)(1)(-2) = 2A \Rightarrow A = \frac{1}{2}$

$s = 1$: $2 = B(1)(2)(-1) = -2B \Rightarrow B = -1$

$s = -1$: $2 = C(-1)(-2)(-3) = -6C \Rightarrow C = -\frac{1}{3}$

$s = 2$: $5 = D(2)(1)(3) = 6D \Rightarrow D = \frac{5}{6}$

$\boxed{\mathcal{L}^{-1}\left\{\frac{s^2+1}{s(s-1)(s+1)(s-2)}\right\} = \frac{1}{2} - e^{t} - \frac{1}{3}e^{-t} + \frac{5}{6}e^{2t}}$

---

**Problema 25:** $\mathcal{L}^{-1}\left\{\frac{1}{s^3+5s}\right\}$

$\frac{1}{s^3+5s} = \frac{1}{s(s^2+5)} = \frac{A}{s} + \frac{Bs+C}{s^2+5}$

$1 = A(s^2+5) + (Bs+C)s$

$s = 0$: $1 = 5A \Rightarrow A = \frac{1}{5}$

Coef. $s^2$: $0 = A + B \Rightarrow B = -\frac{1}{5}$

Coef. $s$: $0 = C$

$\frac{1}{s^3+5s} = \frac{1}{5s} - \frac{s}{5(s^2+5)}$

$\boxed{\mathcal{L}^{-1}\left\{\frac{1}{s^3+5s}\right\} = \frac{1}{5} - \frac{1}{5}\cos(\sqrt{5}t)}$

---

**Problema 26:** $\mathcal{L}^{-1}\left\{\frac{s}{(s+2)(s^2+4)}\right\}$

$\frac{s}{(s+2)(s^2+4)} = \frac{A}{s+2} + \frac{Bs+C}{s^2+4}$

$s = A(s^2+4) + (Bs+C)(s+2)$

$s = -2$: $-2 = A(8) \Rightarrow A = -\frac{1}{4}$

Coef. $s^2$: $0 = A + B \Rightarrow B = \frac{1}{4}$

Coef. $s^0$: $0 = 4A + 2C \Rightarrow C = \frac{1}{2}$

$\boxed{\mathcal{L}^{-1}\left\{\frac{s}{(s+2)(s^2+4)}\right\} = -\frac{1}{4}e^{-2t} + \frac{1}{4}\cos(2t) + \frac{1}{4}\sin(2t)}$

---

**Problema 27:** $\mathcal{L}^{-1}\left\{\frac{2s-4}{(s^2+s)(s^2+1)}\right\}$

$= \frac{2s-4}{s(s+1)(s^2+1)} = \frac{A}{s} + \frac{B}{s+1} + \frac{Cs+D}{s^2+1}$

$s = 0$: $-4 = A(1)(1) \Rightarrow A = -4$

$s = -1$: $-6 = B(-1)(2) \Rightarrow B = 3$

Expandiendo y comparando: $C = 1$, $D = 3$

$\boxed{\mathcal{L}^{-1}\left\{\frac{2s-4}{(s^2+s)(s^2+1)}\right\} = -4 + 3e^{-t} + \cos(t) + 3\sin(t)}$

---

**Problema 28:** $\mathcal{L}^{-1}\left\{\frac{1}{s^4-9}\right\}$

$s^4 - 9 = (s^2-3)(s^2+3)$

$\frac{1}{(s^2-3)(s^2+3)} = \frac{As+B}{s^2-3} + \frac{Cs+D}{s^2+3}$

$1 = (As+B)(s^2+3) + (Cs+D)(s^2-3)$

Coef. $s^3$: $A + C = 0$, Coef. $s^2$: $B + D = 0$

Coef. $s$: $3A - 3C = 0 \Rightarrow A = C = 0$

Coef. $s^0$: $3B - 3D = 1$

De $B + D = 0$ y $3B - 3D = 1$: $B = \frac{1}{6}$, $D = -\frac{1}{6}$

$\boxed{\mathcal{L}^{-1}\left\{\frac{1}{s^4-9}\right\} = \frac{1}{6\sqrt{3}}\sinh(\sqrt{3}t) - \frac{1}{6\sqrt{3}}\sin(\sqrt{3}t)}$

---

**Problema 29:** $\mathcal{L}^{-1}\left\{\frac{1}{(s^2+1)(s^2+4)}\right\}$

$\frac{1}{(s^2+1)(s^2+4)} = \frac{As+B}{s^2+1} + \frac{Cs+D}{s^2+4}$

$1 = (As+B)(s^2+4) + (Cs+D)(s^2+1)$

Coef. $s^3$: $A + C = 0$, Coef. $s^2$: $B + D = 0$

Coef. $s$: $4A + C = 0 \Rightarrow A = C = 0$

Coef. $s^0$: $4B + D = 1$

De $B + D = 0$ y $4B + D = 1$: $3B = 1 \Rightarrow B = \frac{1}{3}$, $D = -\frac{1}{3}$

$\boxed{\mathcal{L}^{-1}\left\{\frac{1}{(s^2+1)(s^2+4)}\right\} = \frac{1}{3}\sin(t) - \frac{1}{6}\sin(2t)}$

---

**Problema 30:** $\mathcal{L}^{-1}\left\{\frac{6s+3}{s^4+5s^2+4}\right\}$

$s^4+5s^2+4 = (s^2+1)(s^2+4)$

$\frac{6s+3}{(s^2+1)(s^2+4)} = \frac{As+B}{s^2+1} + \frac{Cs+D}{s^2+4}$

$6s+3 = (As+B)(s^2+4) + (Cs+D)(s^2+1)$

Coef. $s^3$: $A + C = 0$, Coef. $s^2$: $B + D = 0$

Coef. $s$: $4A + C = 6 \Rightarrow 3A = 6 \Rightarrow A = 2$, $C = -2$

Coef. $s^0$: $4B + D = 3$

De $B + D = 0$ y $4B + D = 3$: $3B = 3 \Rightarrow B = 1$, $D = -1$

$\frac{6s+3}{(s^2+1)(s^2+4)} = \frac{2s+1}{s^2+1} + \frac{-2s-1}{s^2+4}$

$\boxed{\mathcal{L}^{-1}\left\{\frac{6s+3}{s^4+5s^2+4}\right\} = 2\cos(t) + \sin(t) - 2\cos(2t) - \frac{1}{2}\sin(2t)}$

\end{document}
